# 2020732077_양봉윤_HW_3  
---
# P3.1  
$\text{상태변수 설정}$  
$x_1(t) = y(t) \ , \ x_2(t) = \frac{d y(t)}{dt}$  

$[운동방정식]$  
$M \cdot \frac{d^2 y(t)}{dt^2} = F(t) - b \cdot \frac{d y(t)}{dt} - k y(t)$  

$\text{[상태변수로 1차미분방정식 표현]}$  
$M \cdot \dot{x_2}(t))  = F(t) - b x_2(t) - k x_1(t)$   
$\dot{x_2}(t) = \frac{-k}{M} \dot{x_1}(t) - \frac{b}{M} x_2(t) + \frac{1}{M} F(t)$
 
$[상태미분방정식]$  

$$ \dot{x}(t) = \begin{vmatrix} 0 && 1 \\
-\frac{k}{M} && -\frac{b}{M} \end{vmatrix} x(t) + \begin{vmatrix} 0 \\
\frac{1}{M} \end{vmatrix}F(t) $$

$$y(t) = \begin{vmatrix} 1 && 0 \end{vmatrix}$$


--- 
# P3.3  
$[상태변수 설정]$  
$x_1(t) = i_L(t) \ , \ x_2(t) = v_c(t)$  

$*KCL 사용$  
$i_L(t) = x_1(t) = \frac{v_2(t) - x_2(t)}{R} - C \cdot \frac{d V_c(t)}{dt} $  
$\frac{d V_c(t)}{dt} = \frac{-1}{C} \cdot {x_1(t) + \frac{v_2(t) - x_2(t)}{R}}$  

$*KVL 사용$  
$-V_1(t) + L \cdot \frac{d i_L(t)}{dt} - v_c(t) + v_2(t) = 0 $  
$\frac{d i_L(t)}{dt} = v_1(t) - v_2(t) + v_c(t)$  

$[상태미분방정식]$

$$\dot{x}(t) = \begin{bmatrix} 0 & \frac{1}{L} \\
-\frac{1}{C} & -\frac{1}{RC} \end{bmatrix} \mathbf{x}(t) + \begin{bmatrix} \frac{1}{L} && -\frac{1}{L} \\
0 && \frac{1}{RC} \end{bmatrix} V(t)$$

---
# P3.5  
$\text{[폐루프 전달함수 T(s)]}$  
$T(s) = \frac{Y(s)}{R(s)}$  
$Y(s) = G(s){R(s)-Y(s)}$  
$Y(s){G(s)+1} = G(s)R(s)$  

$*\text{T(s)를 G(s)에 대한 식으로 정리, 블록도를 이용하여 구한 G(s) 대입}$  
$T(s) = \frac{Y(s)}{R(s)} = \frac{G(s)}{G(s)+1} = \frac{S+2}{S^3+5S^2-23S+2}$  

$*\text{상태변수 모델을 구하고 위상변수형 블록선도 작성}$  
$T(s) = \frac{Y(s)}{R(s)} = \frac{G(s)}{G(s)+1} = \frac{S+2}{S^3+5S^2-23S+2} \cdot \frac{Z(s)}{Z(s)}$  
$Y(s) = (S+2)Z(s)$  
$R(s) = (S^3 + 5S^2 -23S +2)Z(s)$  
$라플라스역변환$  
$y(t) = \dot{z}{t} + 2z(t)$  
$r(t) = \dddot{z}{t} + 5\ddot{z}{t} - 23\dot{z}{t} + 2z(t)$  
$\dddot{z}{t} = -5\ddot{z}{t} + 23\dot{z}{t} - 2z(t) +r(t)$  

$$\begin{pmatrix} x_1(t) \\
x_2(t) \\
x_3(t) \end{pmatrix} = \begin{pmatrix} z(t) \\
\dot{x_1}(t) \\
\dot{x_2}(t) \end{pmatrix} = \begin{pmatrix} z(t) \\
\dot{z}(t) \\
\ddot{z}(t) \end{pmatrix}$$

$$\dot{x}(t) = \begin{pmatrix} 0 & 1 & 0 \\
0 & 0 & 1 \\
-2 & 23 & -5 \end{pmatrix} x(t) + \begin{pmatrix} 0 \\  
0 \\
1 \end{pmatrix} r(t)$$

$$y(t) = \begin{pmatrix} 2 & 1 & 0 \end{pmatrix} x(t)$$

---
# P3.12  
$*\text{상태변수 모델}$  
$\frac{Y(s)}{R(s)} \cdot \frac {Z(s)}{Z(s)}$  
$Y(s) = 8(s+5)Z(S) \  \, \ R(s) = (S^3 +12S^2 +44S + 48)Z(s)$  
$라플라스역변환$   
$y(t) = 40z(t) + 8 \dot{z}{t}$  
$r(t) = 48z(t) + 44 \dot{z}{t} + 12\ddot{z}{t} + \dddot{z}{t}$  
$\dddot{z}{t} = r(t) = 48z(t) -44 \dot{z}{t} -12 \ddot{z}{t}$  

$$\dot{x}(t) = \begin{pmatrix} 0 & 1 & 0 \\
0 & 0 & 1 \\
-44 & -44 & -12 \end{pmatrix} x(t) + \begin{pmatrix} 0 \\
0 \\
1 \end{pmatrix} r(t)$$  

$$y(t) = \begin{pmatrix} 40 & 8 & 0 \end{pmatrix} x(t)$$  

$\Phi(t) = \mathcal{L}^{-1} \left( \Phi(s) \right) = \mathcal{L}^{-1} \left( (sI - A)^{-1} \right)$


---
# P 3.17  
$\dot{x}{t} = Ax(t) + Bu(t)$  
$y(t) = Cx(t) +Du(t)$  

$s X(s) = A X(s) + B U(s)$  
$X(s)(s I - A) = B U(s)\ ,\ \  X(s) = (s I - A)^{-1} B U(s)$

$Y(s) = C X(s) + D U(s)$  
$Y(s) = C (s I - A)^{-1} B U(s) + D U(s)$  

$\frac{Y(s)}{U(s)} = C (s I - A)^{-1} B + D$  
$\frac{Y(s)}{U(s)} = \frac{4(s - 3)}{s^3 - 14s^2 + 37s + 20}$

